DeBruijnSSA/BinSyntax/Rewrite/Region/Cong.lean
@@ -1,0 +1,261 @@
+import DeBruijnSSA.BinSyntax.Typing.Region
+import DeBruijnSSA.BinSyntax.Syntax.Rewrite
+
+import Discretion.Utils.Quotient
+
+namespace BinSyntax
+
+variable [Φ: EffInstSet φ (Ty α) ε] [PartialOrder α] [SemilatticeSup ε] [OrderBot ε]
+
+namespace Region
+
+inductive WfD.CongD (P : Ctx α ε → LCtx α → Region φ → Region φ → Sort _)
+  : Ctx α ε → LCtx α → Region φ → Region φ → Sort _
+  | case_left : e.WfD Γ ⟨Ty.coprod A B, ⊥⟩ → CongD P (⟨A, ⊥⟩::Γ) L r r' → s.WfD (⟨B, ⊥⟩::Γ) L
+    → CongD P Γ L (Region.case e r s) (Region.case e r' s)
+  | case_right : e.WfD Γ ⟨Ty.coprod A B, ⊥⟩ → r.WfD (⟨A, ⊥⟩::Γ) L → CongD P (⟨B, ⊥⟩::Γ) L s s'
+    → CongD P Γ L (Region.case e r s) (Region.case e r s')
+  | let1 : e.WfD Γ ⟨A, e'⟩ → CongD P (⟨A, ⊥⟩::Γ) L r r'
+    → CongD P Γ L (Region.let1 e r) (Region.let1 e r')
+  | let2 : e.WfD Γ ⟨Ty.prod A B, e'⟩ → CongD P (⟨B, ⊥⟩::⟨A, ⊥⟩::Γ) L r r'
+    → CongD P Γ L (Region.let2 e r) (Region.let2 e r')
+  | cfg_entry (R : LCtx α) :
+    (hR : R.length = n) →
+    CongD P Γ (R ++ L) β β' →
+    (∀i : Fin n, (G i).WfD (⟨R.get (i.cast hR.symm), ⊥⟩::Γ) (R ++ L)) →
+    CongD P Γ L (Region.cfg β n G) (Region.cfg β' n G)
+  | cfg_block (R : LCtx α) :
+    (hR : R.length = n) →
+    β.WfD Γ (R ++ L) →
+    (hG : ∀i : Fin n, (G i).WfD (⟨R.get (i.cast hR.symm), ⊥⟩::Γ) (R ++ L)) →
+    (i : Fin n) →
+    CongD P (⟨R.get (i.cast hR.symm), ⊥⟩::Γ) (R ++ L) (G i) g' →
+    CongD P Γ L (Region.cfg β n G) (Region.cfg β n (Function.update G i g'))
+  | rel : P Γ L r r' → CongD P Γ L r r'
+
+def WfD.CongD.left {P : Ctx α ε → LCtx α → Region φ → Region φ → Sort _} {Γ L r r'}
+  (toLeft : ∀{Γ L r r'}, P Γ L r r' → r.WfD Γ L) : CongD P Γ L r r' → r.WfD Γ L
+  | case_left de pr ds => case de (pr.left toLeft) ds
+  | case_right de dr ps => case de dr (ps.left toLeft)
+  | let1 de pr => WfD.let1 de (pr.left toLeft)
+  | let2 de pr => WfD.let2 de (pr.left toLeft)
+  | cfg_entry R hR pβ dG => WfD.cfg _ R hR (pβ.left toLeft) dG
+  | cfg_block R hR dβ dG i pr => WfD.cfg _ R hR dβ (λk => by
+    if h : k = i then
+      cases h
+      exact (pr.left toLeft)
+    else
+      exact dG k
+  )
+  | rel p => toLeft p
+
+def WfD.CongD.right {P : Ctx α ε → LCtx α → Region φ → Region φ → Sort _} {Γ L r r'}
+  (toRight : ∀{Γ L r r'}, P Γ L r r' → r'.WfD Γ L) : CongD P Γ L r r' → r'.WfD Γ L
+  | case_left de pr ds => case de (pr.right toRight) ds
+  | case_right de dr ps => case de dr (ps.right toRight)
+  | let1 de pr => WfD.let1 de (pr.right toRight)
+  | let2 de pr => WfD.let2 de (pr.right toRight)
+  | cfg_entry R hR pβ dG => WfD.cfg _ R hR (pβ.right toRight) dG
+  | cfg_block R hR dβ dG i pr => WfD.cfg _ R hR dβ (λk => by
+    if h : k = i then
+      cases h
+      simp only [Function.update_same]
+      exact (pr.right toRight)
+    else
+      simp only [ne_eq, h, not_false_eq_true, Function.update_noteq]
+      exact dG k
+  )
+  | rel p => toRight p
+
+inductive Wf.Cong (P : Ctx α ε → LCtx α → Region φ → Region φ → Prop)
+  : Ctx α ε → LCtx α → Region φ → Region φ → Prop
+  | case_left : e.Wf Γ ⟨Ty.coprod A B, e'⟩ → Cong P (⟨A, ⊥⟩::Γ) L r r' → s.Wf (⟨B, ⊥⟩::Γ) L
+    → Cong P Γ L (Region.case e r s) (Region.case e r' s)
+  | case_right : e.Wf Γ ⟨Ty.coprod A B, e'⟩ → r.Wf (⟨A, ⊥⟩::Γ) L → Cong P (⟨B, ⊥⟩::Γ) L s s'
+    → Cong P Γ L (Region.case e r s) (Region.case e r s')
+  | let1 : a.Wf Γ ⟨A, e⟩ → Cong P (⟨A, ⊥⟩::Γ) L r r'
+    → Cong P Γ L (Region.let1 a r) (Region.let1 a r')
+  | let2 : a.Wf Γ ⟨Ty.prod A B, e⟩ → Cong P (⟨B, ⊥⟩::⟨A, ⊥⟩::Γ) L r r'
+    → Cong P Γ L (Region.let2 a r) (Region.let2 a r')
+  | cfg_entry (R : LCtx α) :
+    (hR : R.length = n) →
+    Cong P Γ (R ++ L) β β' →
+    (∀i : Fin n, (G i).Wf (⟨R.get (i.cast hR.symm), ⊥⟩::Γ) (R ++ L)) →
+    Cong P Γ L (Region.cfg β n G) (Region.cfg β' n G)
+  | cfg_block (R : LCtx α) :
+    (hR : R.length = n) →
+    β.Wf Γ (R ++ L) →
+    (hG : ∀i : Fin n, (G i).Wf (⟨R.get (i.cast hR.symm), ⊥⟩::Γ) (R ++ L)) →
+    (i : Fin n) →
+    Cong P (⟨R.get (i.cast hR.symm), ⊥⟩::Γ) (R ++ L) (G i) g' →
+    Cong P Γ L (Region.cfg β n G) (Region.cfg β n (Function.update G i g'))
+  | rel : P Γ L r r' → Cong P Γ L r r'
+
+theorem Wf.Cong.left {P : Ctx α ε → LCtx α → Region φ → Region φ → Prop} {Γ L r r'}
+  (toLeft : ∀{Γ L r r'}, P Γ L r r' → r.Wf Γ L) : Wf.Cong P Γ L r r' → r.Wf Γ L
+  | case_left de pr ds => case de (pr.left toLeft) ds
+  | case_right de dr ps => case de dr (ps.left toLeft)
+  | let1 de pr => Wf.let1 de (pr.left toLeft)
+  | let2 de pr => Wf.let2 de (pr.left toLeft)
+  | cfg_entry R hR pβ dG => Wf.cfg _ R hR (pβ.left toLeft) dG
+  | cfg_block R hR dβ dG i pr => Wf.cfg _ R hR dβ (λk => by
+    if h : k = i then
+      cases h
+      exact (pr.left toLeft)
+    else
+      exact dG k
+  )
+  | rel p => toLeft p
+
+theorem Wf.Cong.right {P : Ctx α ε → LCtx α → Region φ → Region φ → Prop} {Γ L r r'}
+  (toRight : ∀{Γ L r r'}, P Γ L r r' → r'.Wf Γ L) : Wf.Cong P Γ L r r' → r'.Wf Γ L
+  | case_left de pr ds => case de (pr.right toRight) ds
+  | case_right de dr ps => case de dr (ps.right toRight)
+  | let1 de pr => Wf.let1 de (pr.right toRight)
+  | let2 de pr => Wf.let2 de (pr.right toRight)
+  | cfg_entry R hR pβ dG => Wf.cfg _ R hR (pβ.right toRight) dG
+  | cfg_block R hR dβ dG i pr => Wf.cfg _ R hR dβ (λk => by
+    if h : k = i then
+      cases h
+      simp only [Function.update_same]
+      exact (pr.right toRight)
+    else
+      simp only [ne_eq, h, not_false_eq_true, Function.update_noteq]
+      exact dG k
+  )
+  | rel p => toRight p
+
+theorem Wf.Cong.vwk {P : Ctx α ε → LCtx α → Region φ → Region φ → Prop}
+  (toVwk : ∀Γ Δ L r r' ρ, Γ.Wkn Δ ρ → P Δ L r r' → P Γ L (r.vwk ρ) (r'.vwk ρ))
+  {Γ L r r'}
+  {ρ : ℕ → ℕ} (hρ : Γ.Wkn Δ ρ)
+  : Wf.Cong P Δ L r r' → Wf.Cong P Γ L (r.vwk ρ) (r'.vwk ρ)
+  | case_left de pr ds => case_left (de.wk hρ) (pr.vwk toVwk hρ.slift) (ds.vwk hρ.slift)
+  | case_right de dr ps => case_right (de.wk hρ) (dr.vwk hρ.slift) (ps.vwk toVwk hρ.slift)
+  | let1 de pr => let1 (de.wk hρ) (pr.vwk toVwk hρ.slift)
+  | let2 de pr => let2 (de.wk hρ) (pr.vwk toVwk hρ.sliftn₂)
+  | cfg_entry R hR pβ dG => cfg_entry R hR (pβ.vwk toVwk hρ) (λi => (dG i).vwk hρ.slift)
+  | cfg_block R hR dβ dG i pr => by
+    simp only [Region.vwk, Function.comp_update_apply]
+    exact cfg_block R hR (dβ.vwk hρ) (λi => (dG i).vwk hρ.slift) i (pr.vwk toVwk hρ.slift)
+  | rel p => rel $ toVwk _ _ _ _ _ _ hρ p
+
+-- TODO: Wf.Cong.lwk
+
+theorem Wf.Cong.eqv_iff {P : Ctx α ε → LCtx α → Region φ → Region φ → Prop} {Γ L r r'}
+  (toLeft : ∀{Γ L r r'}, P Γ L r r' → r.Wf Γ L)
+  (toRight : ∀{Γ L r r'}, P Γ L r r' → r'.Wf Γ L)
+  (p : EqvGen (Wf.Cong P Γ L) r r') : r.Wf Γ L ↔ r'.Wf Γ L
+  := by induction p with
+  | rel _ _ h => exact ⟨λ_ => h.right toRight, λ_ => h.left toLeft⟩
+  | refl => rfl
+  | symm _ _ _ I => exact I.symm
+  | trans _ _ _ _ _ Il Ir => exact Il.trans Ir
+
+theorem Wf.Cong.case_left_eqv
+  {P : Ctx α ε → LCtx α → Region φ → Region φ → Prop} {r r' s : Region φ}
+  (he : e.Wf Γ ⟨Ty.coprod A B, e'⟩)
+  (p : EqvGen (Wf.Cong P (⟨A, ⊥⟩::Γ) L) r r')
+  (hs : s.Wf (⟨B, ⊥⟩::Γ) L)
+  : EqvGen (Wf.Cong P Γ L) (Region.case e r s) (Region.case e r' s)
+  := by induction p with
+  | rel _ _ h => exact EqvGen.rel _ _ (h.case_left he hs)
+  | refl _ => exact EqvGen.refl _
+  | symm _ _ _ I => exact I.symm
+  | trans _ _ _ _ _ Il Ir => exact Il.trans _ _ _ Ir
+
+theorem Wf.Cong.case_right_eqv
+  {P : Ctx α ε → LCtx α → Region φ → Region φ → Prop} {r s s' : Region φ}
+  (he : e.Wf Γ ⟨Ty.coprod A B, e'⟩)
+  (hr : r.Wf (⟨A, ⊥⟩::Γ) L)
+  (p : EqvGen (Wf.Cong P (⟨B, ⊥⟩::Γ) L) s s')
+  : EqvGen (Wf.Cong P Γ L) (Region.case e r s) (Region.case e r s')
+  := by induction p with
+  | rel _ _ h => exact EqvGen.rel _ _ (h.case_right he hr)
+  | refl _ => exact EqvGen.refl _
+  | symm _ _ _ I => exact I.symm
+  | trans _ _ _ _ _ Il Ir => exact Il.trans _ _ _ Ir
+
+theorem Wf.Cong.let1_eqv
+  {P : Ctx α ε → LCtx α → Region φ → Region φ → Prop}
+  {a : Term φ} (ha : a.Wf Γ ⟨A, e⟩)
+  (p : EqvGen (Wf.Cong P (⟨A, ⊥⟩::Γ) L) r r')
+  : EqvGen (Wf.Cong P Γ L) (Region.let1 a r) (Region.let1 a r')
+  := by induction p with
+  | rel _ _ h => exact EqvGen.rel _ _ (h.let1 ha)
+  | refl _ => exact EqvGen.refl _
+  | symm _ _ _ I => exact I.symm
+  | trans _ _ _ _ _ Il Ir => exact Il.trans _ _ _ Ir
+
+theorem Wf.Cong.let2_eqv
+  {P : Ctx α ε → LCtx α → Region φ → Region φ → Prop}
+  {a : Term φ} (ha : a.Wf Γ ⟨Ty.prod A B, e⟩)
+  (p : EqvGen (Wf.Cong P (⟨B, ⊥⟩::⟨A, ⊥⟩::Γ) L) r r')
+  : EqvGen (Wf.Cong P Γ L) (Region.let2 a r) (Region.let2 a r')
+  := by induction p with
+  | rel _ _ h => exact EqvGen.rel _ _ (h.let2 ha)
+  | refl _ => exact EqvGen.refl _
+  | symm _ _ _ I => exact I.symm
+  | trans _ _ _ _ _ Il Ir => exact Il.trans _ _ _ Ir
+
+theorem Wf.Cong.cfg_entry_eqv
+  {P : Ctx α ε → LCtx α → Region φ → Region φ → Prop}
+  (R : LCtx α) (hR : R.length = n)
+  (p : EqvGen (Wf.Cong P Γ (R ++ L)) β β')
+  (dG : ∀i : Fin n, (G i).Wf (⟨R.get (i.cast hR.symm), ⊥⟩::Γ) (R ++ L))
+  : EqvGen (Wf.Cong P Γ L) (Region.cfg β n G) (Region.cfg β' n G)
+  := by induction p with
+  | rel _ _ h => exact EqvGen.rel _ _ (h.cfg_entry R hR dG)
+  | refl _ => exact EqvGen.refl _
+  | symm _ _ _ I => exact I.symm
+  | trans _ _ _ _ _ Il Ir => exact Il.trans _ _ _ Ir
+
+theorem Wf.Cong.cfg_block_eqv
+  {P : Ctx α ε → LCtx α → Region φ → Region φ → Prop}
+  (R : LCtx α) (hR : R.length = n)
+  (β)
+  (dβ : β.Wf Γ (R ++ L))
+  (dG : ∀i : Fin n, (G i).Wf (⟨R.get (i.cast hR.symm), ⊥⟩::Γ) (R ++ L))
+  (i : Fin n)
+  (p : EqvGen (Wf.Cong P (⟨R.get (i.cast hR.symm), ⊥⟩::Γ) (R ++ L)) (G i) g')
+  (toLeft : ∀{Γ L r r'}, P Γ L r r' → r.Wf Γ L)
+  (toRight : ∀{Γ L r r'}, P Γ L r r' → r'.Wf Γ L)
+  : EqvGen (Wf.Cong P Γ L) (Region.cfg β n G) (Region.cfg β n (Function.update G i g'))
+  := by
+  generalize hg : G i = g
+  rw [hg] at p
+  induction p generalizing G with
+  | rel _ _ h => exact EqvGen.rel _ _ $ (hg ▸ h).cfg_block _ hR dβ dG i
+  | refl _ =>
+    rw [<-hg, Function.update_eq_self]
+    exact EqvGen.refl _
+  | symm x y hxy I =>
+    have I := @I (Function.update G i x)
+    rw [Function.update_idem, <-hg, Function.update_eq_self] at I
+    apply (I _ (by simp)).symm
+    intro k
+    if h : k = i then
+      cases h
+      rw [Function.update_same]
+      apply (eqv_iff toLeft toRight hxy).mpr
+      rw [<-hg]
+      apply dG
+    else
+      rw [Function.update_noteq h]
+      exact dG k
+  | trans x y z hxy _ Il Ir =>
+    apply EqvGen.trans _ _ _ (Il dG hg)
+    have h : Function.update G i z = Function.update (Function.update G i y) i z
+      := by simp
+    rw [h]
+    apply Ir _ (by simp)
+    intro k
+    if h : k = i then
+      cases h
+      rw [Function.update_same]
+      apply (eqv_iff toLeft toRight hxy).mp
+      rw [<-hg]
+      apply dG
+    else
+      rw [Function.update_noteq h]
+      exact dG k
