DeBruijnSSA/BinSyntax/Typing/BBRegion/VSubst.lean
@@ -1,0 +1,15 @@
+import DeBruijnSSA.BinSyntax.Typing.BBRegion.Basic
+import DeBruijnSSA.BinSyntax.Typing.Block.VSubst
+
+namespace BinSyntax
+
+section Subst
+
+variable
+  [Φ: EffInstSet φ (Ty α) ε] [PartialOrder α] [PartialOrder ε] [Bot ε]
+  {Γ Δ : Ctx α ε} {σ : Term.Subst φ}
+
+def BBRegion.WfD.vsubst {Γ Δ : Ctx α ε} {σ} {r : BBRegion φ} (hσ : σ.WfD Γ Δ)
+  : r.WfD Δ L → (r.vsubst σ).WfD Γ L
+  | cfg n R hR hb hG => cfg n R hR (hb.vsubst hσ)
+    (λi => (hG i).vsubst (hσ.liftn_append_cons' _ (by rw [hb.body.num_defs_eq_length])))
