DeBruijnSSA/BinSyntax/Typing/Block/LSubst.lean
@@ -1,0 +1,16 @@
+import DeBruijnSSA.BinSyntax.Typing.Terminator.LSubst
+import DeBruijnSSA.BinSyntax.Typing.Block.Basic
+
+namespace BinSyntax
+
+section TerminatorSubst
+
+variable
+  [Φ: EffInstSet φ (Ty α) ε] [PartialOrder α] [PartialOrder ε] [OrderBot ε]
+  {Γ Δ : Ctx α ε} {σ : Terminator.Subst φ}
+
+def Block.WfD.lsubst {b : Block φ} (hσ : σ.WfD Γ L K) (hb : b.WfD Γ Ξ L) : (b.lsubst σ).WfD Γ Ξ K
+  where
+  body := hb.body
+  terminator := hb.terminator.lsubst (hσ.vliftn_append'
+    (by rw [hb.body.num_defs_eq_length, Ctx.reverse, List.length_reverse]))
