DeBruijnSSA/BinSyntax/Typing/Block/VSubst.lean
@@ -1,0 +1,18 @@
+import DeBruijnSSA.BinSyntax.Typing.Block.Basic
+import DeBruijnSSA.BinSyntax.Typing.Term.Subst
+import DeBruijnSSA.BinSyntax.Typing.Body.Subst
+import DeBruijnSSA.BinSyntax.Typing.Terminator.VSubst
+
+namespace BinSyntax
+
+section Subst
+
+variable
+  [Φ: EffInstSet φ (Ty α) ε] [PartialOrder α] [PartialOrder ε] [Bot ε]
+  {Γ Δ : Ctx α ε} {σ : Term.Subst φ}
+
+def Block.WfD.vsubst {b : Block φ} (hσ : σ.WfD Γ Δ) (hb : b.WfD Δ Ξ L) : (b.vsubst σ).WfD Γ Ξ L
+  where
+  body := hb.body.subst hσ
+  terminator := hb.terminator.vsubst (hσ.liftn_append'
+    (by rw [hb.body.num_defs_eq_length, Ctx.reverse, List.length_reverse]))
