DeBruijnSSA/BinSyntax/Typing/Body/Subst.lean
@@ -1,0 +1,16 @@
+import DeBruijnSSA.BinSyntax.Typing.Term.Subst
+import DeBruijnSSA.BinSyntax.Typing.Body.Basic
+
+namespace BinSyntax
+
+section Subst
+
+variable
+  [Φ: EffInstSet φ (Ty α) ε] [PartialOrder α] [PartialOrder ε] [Bot ε]
+  {Γ Δ : Ctx α ε} {σ : Term.Subst φ}
+
+def Body.WfD.subst {Γ Δ : Ctx α ε} {σ} {b : Body φ} (hσ : σ.WfD Γ Δ)
+  : b.WfD Δ V → (b.subst σ).WfD Γ V
+  | nil => nil
+  | let1 da dt => let1 (da.subst hσ) (dt.subst hσ.slift)
+  | let2 da dt => let2 (da.subst hσ) (dt.subst hσ.sliftn₂)
