DeBruijnSSA/BinSyntax/Typing/Region/VSubst.lean
@@ -1,0 +1,39 @@
+import DeBruijnSSA.BinSyntax.Typing.Region.Basic
+import DeBruijnSSA.BinSyntax.Typing.Term.Subst
+
+namespace BinSyntax
+
+section Subst
+
+variable
+  [Φ: EffInstSet φ (Ty α) ε] [PartialOrder α] [PartialOrder ε] [Bot ε]
+  {Γ Δ : Ctx α ε} {σ : Term.Subst φ}
+
+def Region.WfD.vsubst {Γ Δ : Ctx α ε} {σ} {r : Region φ} (hσ : σ.WfD Γ Δ)
+  : r.WfD Δ L → (r.vsubst σ).WfD Γ L
+  | br hL ha => br hL (ha.subst hσ)
+  | case he hs ht => case (he.subst hσ) (hs.vsubst hσ.slift) (ht.vsubst hσ.slift)
+  | let1 da dt => let1 (da.subst hσ) (dt.vsubst hσ.slift)
+  | let2 da dt => let2 (da.subst hσ) (dt.vsubst hσ.sliftn₂)
+  | cfg n R hR hr hG => cfg n R hR (hr.vsubst hσ) (λi => (hG i).vsubst hσ.slift)
+
+theorem Region.Wf.vsubst {Γ Δ : Ctx α ε} {σ} {r : Region φ} (hσ : σ.Wf Γ Δ) (h : r.Wf Δ L)
+  : (r.vsubst σ).Wf Γ L
+  := let ⟨d⟩ := h.nonempty; let ⟨hσ⟩ := hσ.nonempty; (d.vsubst hσ).toWf
+
+def Region.InS.vsubst {Γ Δ : Ctx α ε} (σ : Term.Subst.InS φ Γ Δ) (r : InS φ Δ L) : InS φ Γ L
+  := ⟨(r : Region φ).vsubst σ, r.prop.vsubst σ.prop⟩
+
+@[simp]
+theorem Region.InS.coe_vsubst {Γ Δ : Ctx α ε} {σ : Term.Subst.InS φ Γ Δ} {r : InS φ Δ L}
+  : (r.vsubst σ : Region φ) = (r : Region φ).vsubst σ
+  := rfl
+
+theorem Region.InS.vsubst_vsubst {Γ Δ Ξ : Ctx α ε}
+  {σ : Term.Subst.InS φ Γ Δ} {τ : Term.Subst.InS φ Δ Ξ}
+  (r : InS φ Ξ L) : (r.vsubst τ).vsubst σ = r.vsubst (σ.comp τ)
+  := by ext; simp [Region.vsubst_vsubst]
+
+theorem Region.InS.vsubst_equiv {Γ Δ : Ctx α ε} {σ τ : Term.Subst.InS φ Γ Δ}
+  (r : InS φ Δ L) (h : σ ≈ τ) : r.vsubst σ = r.vsubst τ
+  := sorry
