DeBruijnSSA/BinSyntax/Typing/TRegion/LSubst.lean
@@ -1,0 +1,19 @@
+import DeBruijnSSA.BinSyntax.Typing.TRegion.Basic
+import DeBruijnSSA.BinSyntax.Typing.Terminator.LSubst
+import DeBruijnSSA.BinSyntax.Syntax.Subst
+
+namespace BinSyntax
+
+section TerminatorSubst
+
+variable
+  [Φ: EffInstSet φ (Ty α) ε] [PartialOrder α] [PartialOrder ε] [OrderBot ε]
+  {Γ Δ : Ctx α ε} {σ : Terminator.Subst φ}
+
+def TRegion.WfD.lsubst {Γ : Ctx α ε} {L} {σ} {r : TRegion φ} (hσ : σ.WfD Γ L K)
+  : r.WfD Γ L → (r.lsubst σ).WfD Γ K
+  | let1 da dt => let1 da (dt.lsubst hσ.vlift)
+  | let2 da dt => let2 da (dt.lsubst hσ.vliftn₂)
+  | cfg n R hR hr hG => cfg n R hR
+    (hr.lsubst (hσ.liftn_append' hR.symm))
+    (λi => (hG i).lsubst (hσ.liftn_append' hR.symm).vlift)
