DeBruijnSSA/BinSyntax/Typing/TRegion/VSubst.lean
@@ -1,0 +1,16 @@
+import DeBruijnSSA.BinSyntax.Typing.TRegion.Basic
+import DeBruijnSSA.BinSyntax.Typing.Terminator.VSubst
+
+namespace BinSyntax
+
+section Subst
+
+variable
+  [Φ: EffInstSet φ (Ty α) ε] [PartialOrder α] [PartialOrder ε] [Bot ε]
+  {Γ Δ : Ctx α ε} {σ : Term.Subst φ}
+
+def TRegion.WfD.vsubst {Γ Δ : Ctx α ε} {σ}  {r : TRegion φ} (hσ : σ.WfD Γ Δ)
+  : r.WfD Δ L → (r.vsubst σ).WfD Γ L
+  | let1 da dt => let1 (da.subst hσ) (dt.vsubst hσ.slift)
+  | let2 da dt => let2 (da.subst hσ) (dt.vsubst hσ.sliftn₂)
+  | cfg n R hR hr hG => cfg n R hR (hr.vsubst hσ) (λi => (hG i).vsubst hσ.slift)
