DeBruijnSSA/BinSyntax/Typing/Term/Subst.lean
@@ -1,0 +1,265 @@
+import DeBruijnSSA.BinSyntax.Typing.Term.Basic
+import DeBruijnSSA.BinSyntax.Syntax.Subst
+
+namespace BinSyntax
+
+section Subst
+
+variable
+  [Φ: EffInstSet φ (Ty α) ε] [PartialOrder α] [PartialOrder ε] [Bot ε]
+  {Γ Δ : Ctx α ε} {σ : Term.Subst φ}
+
+def Term.Subst.WfD (Γ Δ : Ctx α ε) (σ : Subst φ) : Type _
+  := ∀i : Fin Δ.length, (σ i).WfD Γ (Δ.get i)
+
+def Term.Subst.Wf (Γ Δ : Ctx α ε) (σ : Subst φ) : Prop
+  := ∀i : Fin Δ.length, (σ i).Wf Γ (Δ.get i)
+
+def Term.Subst.InS (φ) [EffInstSet φ (Ty α) ε] (Γ Δ : Ctx α ε) : Type _ := {σ : Subst φ | σ.Wf Γ Δ}
+
+instance Term.Subst.InS.instCoeOut {Γ Δ : Ctx α ε} : CoeOut (Term.Subst.InS φ Γ Δ) (Subst φ)
+  := ⟨λr => r.1⟩
+
+theorem Term.Subst.InS.eq_of_coe_eq {σ τ : Term.Subst.InS φ Γ Δ} (h : (σ : Subst φ) = τ) : σ = τ
+  := by cases σ; cases τ; cases h; rfl
+
+instance Term.Subst.InS.instSetoid {Γ Δ : Ctx α ε} : Setoid (Term.Subst.InS φ Γ Δ) where
+  r σ τ := ∀i, i < Δ.length → σ.val i = τ.val i
+  iseqv := {
+    refl := (λ_ _ _ => rfl)
+    symm := (λh _ hi => (h _ hi).symm)
+    trans := (λhl hr _ hi => (hl _ hi).trans (hr _ hi))
+  }
+
+theorem Term.Subst.Wf.nonempty (hσ : σ.Wf Γ Δ) : Nonempty (σ.WfD Γ Δ)
+  := ⟨λi => Classical.choice (hσ i).nonempty⟩
+
+theorem Term.Subst.WfD.toWf (hσ : σ.WfD Γ Δ) : σ.Wf Γ Δ
+  := λi => (hσ i).toWf
+
+theorem Term.Subst.Wf.nonempty_iff : σ.Wf Γ Δ ↔ Nonempty (σ.WfD Γ Δ)
+  := ⟨Term.Subst.Wf.nonempty, λ⟨h⟩ => h.toWf⟩
+
+def Term.Subst.WfD.lift (h : V ≤ V') (hσ : σ.WfD Γ Δ) : σ.lift.WfD (V::Γ) (V'::Δ)
+  := λi => i.cases (Term.WfD.var (Ctx.Var.head h _)) (λi => (hσ i).wk Ctx.Wkn.id.step)
+
+theorem Term.Subst.Wf.lift (h : V ≤ V') (hσ : σ.Wf Γ Δ) : σ.lift.Wf (V::Γ) (V'::Δ)
+  := λi => i.cases (Term.Wf.var (Ctx.Var.head h _)) (λi => (hσ i).wk Ctx.Wkn.id.step)
+
+def Term.Subst.InS.lift (h : V ≤ V') (σ : InS φ Γ Δ) : InS φ (V::Γ) (V'::Δ)
+  := ⟨Subst.lift σ, σ.prop.lift h⟩
+
+@[simp]
+theorem Term.Subst.coe_lift {h : V ≤ V'} {σ : InS φ Γ Δ}
+  : (σ.lift h : Subst φ) = Subst.lift σ
+  := rfl
+
+def Term.Subst.WfD.slift {head} (hσ : σ.WfD Γ Δ) : σ.lift.WfD (head::Γ) (head::Δ)
+  := hσ.lift (le_refl head)
+
+theorem Term.Subst.Wf.slift {head} (hσ : σ.Wf Γ Δ) : σ.lift.Wf (head::Γ) (head::Δ)
+  := hσ.lift (le_refl head)
+
+def Term.Subst.WfD.lift₂ (h₁ : V₁ ≤ V₁') (h₂ : V₂ ≤ V₂') (hσ : σ.WfD Γ Δ)
+  : σ.lift.lift.WfD (V₁::V₂::Γ) (V₁'::V₂'::Δ)
+  := (hσ.lift h₂).lift h₁
+
+theorem Term.Subst.Wf.lift₂ (h₁ : V₁ ≤ V₁') (h₂ : V₂ ≤ V₂') (hσ : σ.Wf Γ Δ)
+  : σ.lift.lift.Wf (V₁::V₂::Γ) (V₁'::V₂'::Δ)
+  := (hσ.lift h₂).lift h₁
+
+def Term.Subst.WfD.slift₂ {left right} (hσ : σ.WfD Γ Δ)
+  : σ.lift.lift.WfD (left::right::Γ) (left::right::Δ)
+  := hσ.lift₂ (le_refl _) (le_refl _)
+
+theorem Term.Subst.Wf.slift₂ {left right} (hσ : σ.Wf Γ Δ)
+  : σ.lift.lift.Wf (left::right::Γ) (left::right::Δ)
+  := hσ.lift₂ (le_refl _) (le_refl _)
+
+-- TODO: version with nicer defeq?
+def Term.Subst.WfD.liftn_append (Ξ : Ctx α ε) (hσ : σ.WfD Γ Δ)
+  : (σ.liftn Ξ.length).WfD (Ξ ++ Γ) (Ξ ++ Δ) := match Ξ with
+  | [] => by rw [List.nil_append, List.nil_append, List.length_nil, liftn_zero]; exact hσ
+  | A::Ξ => by rw [List.length_cons, liftn_succ]; exact (hσ.liftn_append Ξ).slift
+
+theorem Term.Subst.Wf.liftn_append (Ξ : Ctx α ε) (hσ : σ.Wf Γ Δ)
+  : (σ.liftn Ξ.length).Wf (Ξ ++ Γ) (Ξ ++ Δ) := match Ξ with
+  | [] => by rw [List.nil_append, List.nil_append, List.length_nil, liftn_zero]; exact hσ
+  | A::Ξ => by rw [List.length_cons, liftn_succ]; exact (hσ.liftn_append Ξ).slift
+
+def Term.Subst.WfD.liftn_append' {Ξ : Ctx α ε} (hn : n = Ξ.length) (hσ : σ.WfD Γ Δ)
+  : (σ.liftn n).WfD (Ξ ++ Γ) (Ξ ++ Δ)
+  := hn ▸ hσ.liftn_append Ξ
+
+theorem Term.Subst.Wf.liftn_append' {Ξ : Ctx α ε} (hn : n = Ξ.length) (hσ : σ.Wf Γ Δ)
+  : (σ.liftn n).Wf (Ξ ++ Γ) (Ξ ++ Δ)
+  := hn ▸ hσ.liftn_append Ξ
+
+def Term.Subst.WfD.liftn_append_cons (V) (Ξ : Ctx α ε) (hσ : σ.WfD Γ Δ)
+  : (σ.liftn (Ξ.length + 1)).WfD (V::(Ξ ++ Γ)) (V::(Ξ ++ Δ))
+  := liftn_append (V::Ξ) hσ
+
+theorem Term.Subst.Wf.liftn_append_cons (V) (Ξ : Ctx α ε) (hσ : σ.Wf Γ Δ)
+  : (σ.liftn (Ξ.length + 1)).Wf (V::(Ξ ++ Γ)) (V::(Ξ ++ Δ))
+  := liftn_append (V::Ξ) hσ
+
+def Term.Subst.WfD.liftn_append_cons' (V) {Ξ : Ctx α ε} (hn : n = Ξ.length + 1) (hσ : σ.WfD Γ Δ)
+  : (σ.liftn n).WfD (V::(Ξ ++ Γ)) (V::(Ξ ++ Δ))
+  := hn ▸ hσ.liftn_append_cons V Ξ
+
+theorem Term.Subst.Wf.liftn_append_cons' (V) {Ξ : Ctx α ε} (hn : n = Ξ.length + 1) (hσ : σ.Wf Γ Δ)
+  : (σ.liftn n).Wf (V::(Ξ ++ Γ)) (V::(Ξ ++ Δ))
+  := hn ▸ hσ.liftn_append_cons V Ξ
+
+-- TODO: version with nicer defeq?
+def Term.Subst.WfD.liftn₂ (h₁ : V₁ ≤ V₁') (h₂ : V₂ ≤ V₂') (hσ : σ.WfD Γ Δ)
+  : (σ.liftn 2).WfD (V₁::V₂::Γ) (V₁'::V₂'::Δ)
+  := Subst.liftn_eq_iterate_lift 2 ▸ hσ.lift₂ h₁ h₂
+
+theorem Term.Subst.Wf.liftn₂ (h₁ : V₁ ≤ V₁') (h₂ : V₂ ≤ V₂') (hσ : σ.Wf Γ Δ)
+  : (σ.liftn 2).Wf (V₁::V₂::Γ) (V₁'::V₂'::Δ)
+  := Subst.liftn_eq_iterate_lift 2 ▸ hσ.lift₂ h₁ h₂
+
+def Term.Subst.InS.liftn₂ (h₁ : V₁ ≤ V₁') (h₂ : V₂ ≤ V₂') (σ : Subst.InS φ Γ Δ)
+  : Subst.InS φ (V₁::V₂::Γ) (V₁'::V₂'::Δ)
+  := ⟨Subst.liftn 2 σ, σ.prop.liftn₂ h₁ h₂⟩
+
+theorem Term.Subst.InS.lift_lift (h₁ : V₁ ≤ V₁') (h₂ : V₂ ≤ V₂') (σ : Subst.InS φ Γ Δ)
+  : (σ.lift h₂).lift h₁ = (σ.liftn₂ h₁ h₂)
+  := by simp [lift, liftn₂, Subst.liftn_succ]
+
+def Term.Subst.WfD.sliftn₂ {left right} (hσ : σ.WfD Γ Δ)
+  : (σ.liftn 2).WfD (left::right::Γ) (left::right::Δ)
+  := hσ.liftn₂ (le_refl _) (le_refl _)
+
+theorem Term.Subst.Wf.sliftn₂ {left right} (hσ : σ.Wf Γ Δ)
+  : (σ.liftn 2).Wf (left::right::Γ) (left::right::Δ)
+  := hσ.liftn₂ (le_refl _) (le_refl _)
+
+def Ctx.Var.subst (hσ : σ.WfD Γ Δ) (h : Δ.Var n V) : (σ n).WfD Γ V
+  := (hσ ⟨n, h.length⟩).wk_res h.get
+
+theorem Ctx.Var.subst' (hσ : σ.Wf Γ Δ) (h : Δ.Var n V) : (σ n).Wf Γ V
+  := (hσ ⟨n, h.length⟩).wk_res h.get
+
+def Term.WfD.subst {Γ Δ : Ctx α ε} {σ} (hσ : σ.WfD Γ Δ) {a : Term φ}
+  : a.WfD Δ V → (a.subst σ).WfD Γ V
+  | var h => Ctx.Var.subst hσ h
+  | op df de => op df (de.subst hσ)
+  | let1 da dt => let1 (da.subst hσ) (dt.subst hσ.slift)
+  | pair dl dr => pair (dl.subst hσ) (dr.subst hσ)
+  | let2 da dt => let2 (da.subst hσ) (dt.subst hσ.sliftn₂)
+  | inl d => inl (d.subst hσ)
+  | inr d => inr (d.subst hσ)
+  | case de dl dr => case (de.subst hσ) (dl.subst hσ.slift) (dr.subst hσ.slift)
+  | abort d => abort (d.subst hσ)
+  | unit e => unit e
+
+theorem Term.Wf.subst {a : Term φ} (hσ : σ.Wf Γ Δ) (h : a.Wf Δ V) : (a.subst σ).Wf Γ V
+  := let ⟨d⟩ := h.nonempty; let ⟨hσ⟩ := hσ.nonempty; (d.subst hσ).toWf
+
+
+def Term.InS.subst (σ : Subst.InS φ Γ Δ) (a : InS φ Δ V) : InS φ Γ V
+  := ⟨(a : Term φ).subst σ, a.prop.subst σ.prop⟩
+
+@[simp]
+theorem Term.InS.coe_subst {σ : Subst.InS φ Γ Δ} {a : InS φ Δ V}
+  : (a.subst σ : Term φ) = (a : Term φ).subst σ
+  := rfl
+
+def Term.Subst.InS.get (n) (h : Δ.Var n V) (σ : Subst.InS φ Γ Δ) : Term.InS φ Γ V
+  := ⟨σ.val n, h.subst' σ.prop⟩
+
+@[simp]
+theorem Term.InS.subst_var (σ : Subst.InS φ Γ Δ) (h : Δ.Var n V) :
+  (var n h).subst σ = σ.get n h
+  := rfl
+
+@[simp]
+theorem Term.InS.subst_op (σ : Subst.InS φ Γ Δ) (df : Φ.EFn f A B e) (de : InS φ Δ ⟨A, e⟩) :
+  (op f df de).subst σ = op f df (de.subst σ)
+  := rfl
+
+@[simp]
+theorem Term.InS.subst_pair (σ : Subst.InS φ Γ Δ) (dl : InS φ Δ ⟨A, e⟩) (dr : InS φ Δ ⟨B, e⟩) :
+  (pair dl dr).subst σ = pair (dl.subst σ) (dr.subst σ)
+  := rfl
+
+@[simp]
+theorem Term.InS.subst_inl (σ : Subst.InS φ Γ Δ) (d : InS φ Δ ⟨A, e⟩) :
+  (inl (right := right) d).subst σ = inl (d.subst σ)
+  := rfl
+
+@[simp]
+theorem Term.InS.subst_inr (σ : Subst.InS φ Γ Δ) (d : InS φ Δ ⟨B, e⟩) :
+  (inr (left := left) d).subst σ = inr (d.subst σ)
+  := rfl
+
+@[simp]
+theorem Term.InS.subst_abort (σ : Subst.InS φ Γ Δ) (d : InS φ Δ ⟨Ty.empty, e⟩) :
+  (abort (tyOut := tyOut) d).subst σ = abort (tyOut := tyOut) (d.subst σ)
+  := rfl
+
+@[simp]
+theorem Term.InS.subst_unit (σ : Subst.InS φ Γ Δ) (e : ε) :
+  (unit e).subst σ = unit e
+  := rfl
+
+theorem Term.InS.subst_equiv {σ τ : Subst.InS φ Γ Δ} (a : InS φ Δ V)
+  (h : σ ≈ τ) : a.subst σ = a.subst τ
+  := sorry
+
+def Term.WfD.subst0 {a : Term φ} (ha : a.WfD Δ V) : a.subst0.WfD Δ (V::Δ)
+  := λi => i.cases ha (λi => Term.WfD.var ⟨by simp, by simp⟩)
+
+theorem Term.Wf.subst0 {a : Term φ} (ha : a.Wf Δ V) : a.subst0.Wf Δ (V::Δ)
+  := λi => i.cases ha (λi => Term.Wf.var ⟨by simp, by simp⟩)
+
+def Term.InS.subst0 (a : InS φ Γ V) : Subst.InS φ Γ (V::Γ)
+  := ⟨(a : Term φ).subst0, a.prop.subst0⟩
+
+@[simp]
+theorem Term.InS.coe_subst0 {a : InS φ Γ V}
+  : (a.subst0 : Subst φ) = (a : Term φ).subst0
+  := rfl
+
+@[simp]
+theorem Term.Subst.InS.get_0_subst0 (a : Term.InS φ Δ ty)
+  : a.subst0.get 0 (by simp) = a
+  := rfl
+
+@[simp]
+theorem Term.Subst.InS.get_succ_lift (n)
+  (h : Ctx.Var _ (n + 1) ty) (σ : Subst.InS φ Γ Δ)
+  (hv : lo ≤ hi)
+  : (σ.lift hv).get (n + 1) h = (σ.get n h.tail).wk ⟨Nat.succ, by simp⟩
+  := rfl
+
+def Term.Subst.WfD.comp {Γ Δ Ξ : Ctx α ε} {σ : Term.Subst φ} {τ : Term.Subst φ}
+  (hσ : σ.WfD Γ Δ) (hτ : τ.WfD Δ Ξ) : (σ.comp τ).WfD Γ Ξ
+  := λi => (hτ i).subst hσ
+
+theorem Term.Subst.Wf.comp {Γ Δ Ξ : Ctx α ε} {σ : Term.Subst φ} {τ : Term.Subst φ}
+  (hσ : σ.Wf Γ Δ) (hτ : τ.Wf Δ Ξ) : (σ.comp τ).Wf Γ Ξ
+  := λi => (hτ i).subst hσ
+
+def Term.Subst.InS.comp {Γ Δ Ξ : Ctx α ε} (σ : Term.Subst.InS φ Γ Δ) (τ : Term.Subst.InS φ Δ Ξ)
+  : Term.Subst.InS φ Γ Ξ
+  := ⟨Subst.comp σ τ, σ.prop.comp τ.prop⟩
+
+@[simp]
+theorem Term.Subst.InS.coe_comp {Γ Δ Ξ : Ctx α ε}
+  {σ : Term.Subst.InS φ Γ Δ} {τ : Term.Subst.InS φ Δ Ξ}
+  : (σ.comp τ : Subst φ) = Subst.comp σ τ
+  := rfl
+
+theorem Term.InS.subst_subst {Γ Δ Ξ : Ctx α ε} {σ : Term.Subst.InS φ Γ Δ} {τ : Term.Subst.InS φ Δ Ξ}
+  (a : InS φ Ξ V) : (a.subst τ).subst σ = a.subst (σ.comp τ)
+  := by ext; simp [Term.subst_subst]
+
+-- TODO: Term.Subst.InS.comp_id, id_comp ==> this is a category!
+
+theorem Term.Subst.InS.comp_assoc {Γ Δ Ξ Ω : Ctx α ε}
+  {σ : Term.Subst.InS φ Γ Δ} {τ : Term.Subst.InS φ Δ Ξ} {υ : Term.Subst.InS φ Ξ Ω}
+  : (σ.comp τ).comp υ = σ.comp (τ.comp υ)
+  := by apply eq_of_coe_eq; simp [Subst.comp_assoc]
