DeBruijnSSA/BinSyntax/Typing/Terminator/VSubst.lean
@@ -1,0 +1,16 @@
+import DeBruijnSSA.BinSyntax.Typing.Terminator.Basic
+import DeBruijnSSA.BinSyntax.Typing.Term.Subst
+import DeBruijnSSA.BinSyntax.Syntax.Subst
+
+namespace BinSyntax
+
+section Subst
+
+variable
+  [Φ: EffInstSet φ (Ty α) ε] [PartialOrder α] [PartialOrder ε] [Bot ε]
+  {Γ Δ : Ctx α ε} {σ : Term.Subst φ}
+
+def Terminator.WfD.vsubst {Γ Δ : Ctx α ε} {σ} {t : Terminator φ} (hσ : σ.WfD Γ Δ)
+  : t.WfD Δ V → (t.vsubst σ).WfD Γ V
+  | br hL ha => br hL (ha.subst hσ)
+  | case he hs ht => case (he.subst hσ) (hs.vsubst hσ.slift) (ht.vsubst hσ.slift)
